UPdated bank

verification_finalised/bank/spares.dfy
@@ -1,18 +1,162 @@
-// Remove unit from the system, this function requires the unit 
-// to be in the system since it does not make sense to remove a unit 
-// which is not there. This function does not preserve the order of the list.
-method RemoveUnit(unit: int)
-requires unit in units;
-ensures |units| == |old(units)| - 1;
-ensures forall i :: (0<=i<|old(units)| && old(units[i]) != unit) ==> old(units[i]) in units; 
-{
-    var key := FindUnitIndex(unit);
-    units := units[..key] + units[(key+1)..];
+// Finds the index of a given unit, if the unit does not exist 
+    // the function returns -1
+    method FindUnitIndex(unit: int) returns (key: int)
+    ensures units == old(units);
+    ensures key == -1 ==> unit !in units;
+    ensures key >=  0 ==> (key < |units| && units[key] == unit);    
+    ensures unit in units ==> (0<=key<|units| && units[key] == unit);
+    {
+        key := -1;
+        var index := 0; var limit := |units|;
+        
+        while index < limit 
+        decreases limit - index;
+        invariant index <= limit;
+        invariant key == -1 ==> unit !in units[..index];
+        invariant key >=  0 ==> (key < |units| && units[key] == unit);
+        {
+            if unit == units[index] { key := index; }
+            index := index + 1;
+        }
+    }
+
+    // Remove unit from the system by index, this function requires the unit 
+    // to be in the system since it does not make sense to remove a unit 
+    // which is not there. This function preserves the order of the list.
+    method RemoveUnitByIndex(index: int)
+    requires 0<=index<|units|;
+    ensures units == old(units[..index]) + old(units[(index+1)..]);
+    {
+        units := units[..index] + units[(index+1)..];
+    }
+
+    // GetAvailableUnits takes a criterion c and a number of blood units n and determines whether 
+    // the blood bank has enough units satisfying the criterion. The criterion is the same as specified 
+    // for OrderUnits
+    method GetAvailableUnits(c: int) returns (res: seq<int>)
+    requires c != 0;
+    ensures units == old(units);
+    ensures forall i :: 0<=i<|res| ==> res[i]%c == 0;
+    ensures forall i :: 0<=i<|units| ==> units[i]%c == 0 ==> units[i] in res;
+    {
+        var index, limit := 0, |units|;  
+        res := [];
+        while index < limit
+        decreases limit - index;
+        invariant index <= limit;
+        invariant forall i :: 0<=i<|res| ==> res[i]%c == 0;
+        invariant forall i :: 0<=i<index ==> units[i]%c == 0 ==> units[i] in res;
+        {
+            if units[index]%c == 0 { res := res + [units[index]]; }
+            index := index + 1;
+        }
+    }
+
+    // OrderUnits removes the specified number of blood units from the bank which satisfy
+    // a particular criterion. If there are not enough units to meet the specified number, 
+    // the maximum amount available is returned. In the real implementation, the criterion 
+    // may be the type and expiration date of each blood unit. To simulate this criterion with 
+    // integers, the order function will take an integer 'criterion' and all numbers divisible 
+    // by this criterion will be considered 'matches'.
+    // OrderUnits modifies the blood bank units sequence.
+    method OrderUnits(c: int, n: int) returns (results: seq<int>)
+    requires c != 0;
+    ensures |units| == |old(units)| - |results|;
+    ensures forall i, j :: (0<=i<|units| && 0<=j<|units| && i != j) ==> units[i] != units[j];
+    ensures forall i, j :: (0<=i<|results|&& 0<=j<|results| && i != j) ==> results[i] != results[j];
+    ensures forall i :: (i in units ==> i !in results) && (i in results ==> i !in units);
+    {
+        // Variable decleration
+        results := []; var new_units := [];
+        var index, limit, count := 0, |units|, 0;
+
+        // Main loop excecution
+        while index < limit
+        decreases limit - index;
+        invariant index <= limit;
+        invariant |new_units| == |units[..index]| - |results|;
+        invariant forall i :: 0<=i<|results| ==> results[i] in units;
+        invariant forall i :: 0<=i<|new_units| ==> new_units[i] in units;
+        invariant forall i :: index<=i<|units| ==> units[i] !in results && units[i] !in new_units;
+        invariant forall i, j :: (0<=i<|results|&& 0<=j<|results| && i != j) ==> results[i] != results[j];
+        invariant forall i, j :: (0<=i<|new_units|&& 0<=j<|new_units| && i != j) ==> new_units[i] != new_units[j];
+        invariant forall i :: 0<=i<|units[..index]| ==> (units[i] in results && units[i] !in new_units) || (units[i] !in results && units[i] in new_units);
+        {
+            if units[index]%c == 0 && count < n { 
+                results := results + [units[index]]; 
+                count := count + 1; 
+            } else { 
+                new_units := new_units + [units[index]]; 
+            }
+
+            index := index + 1;
+        }
+
+        // Set units equal to new units
+        units := new_units;
+    }
+
+    // FilterUnits returns a sequence of all units in the blood bank which satisfy a particular 
+    // criterion c. The criterion works in the same manner as the criterion for OrderUnits. 
+    // FilterUnits does not modifiy the blood bank units sequence. FilterUnits does not guarantee
+    // the order of the results
+    method FilterUnits(c: int) returns (results: seq<int>)
+    requires c != 0;
+    ensures units == old(units);
+    ensures forall i :: i in results <==> (i%c == 0 && i in units);
+    {
+        results := [];
+        var index, limit := 0, |units|;
+        
+        while index < limit
+        decreases limit - index;
+        invariant index <= limit;
+        invariant forall i :: i in results <==> (i%c == 0 && i in units[..index]);
+        {
+            if units[index]%c == 0 { results := results + [units[index]]; }
+            index := index + 1;
+        }
+    }
 }
 
-// Test 1: 
-bank := new BloodBank();
-bank.AddUnit(1); assert 1 in bank.units;
-bank.AddUnit(2); assert 2 in bank.units;
-bank.RemoveUnit(1); assert 1 !in bank.units; assert 2 in bank.units;
-i2 := bank.FindUnitIndex(2); assert i2 == 0;
+//-----------------------------------------------------------------------------
+// INTEGER INSERT SORT ALGORITHM
+//-----------------------------------------------------------------------------
+
+
+//-----------------------------------------------------------------------------
+// MAIN METHOD TESTING
+//-----------------------------------------------------------------------------
+
+method Main() {
+    // Initialise blood bank and index variables
+    var bank: BloodBank;
+    var i1: int, i2: int, i3: int, i4: int, i5: int;
+    var f1: seq<int>, f2: seq<int>;
+    var available: seq<int>;
+    var order: seq<int>;
+
+    // Test 1: Tests functionality of AddUnit, FindUnitIndex and RemoveUnitByIndex
+    bank := new BloodBank();
+    bank.AddUnit(1); assert bank.units == [1];
+    bank.AddUnit(2); assert bank.units == [1,2];
+    bank.AddUnit(5); assert bank.units == [1,2,5];
+    i2 := bank.FindUnitIndex(2); assert bank.units[i2] == 2;
+    bank.RemoveUnitByIndex(i2); assert bank.units == [1,5];
+    i5 := bank.FindUnitIndex(5); assert bank.units[i5] == 5;
+    bank.RemoveUnitByIndex(i5); assert bank.units == [1];
+    bank.AddUnit(4); assert bank.units == [1,4];
+    bank.AddUnit(2); assert bank.units == [1,4,2];
+    bank.AddUnit(3); assert bank.units == [1,4,2,3];
+    f1 := bank.FilterUnits(2); assert 2 in f1 && 4 in f1 && 1 !in f1 && 3 !in f1;
+    f2 := bank.FilterUnits(3); assert 3 in f2 && 1 !in f2 && 2 !in f2 && 4 !in f2;
+    i2 := bank.FindUnitIndex(2); assert bank.units[i2] == 2;
+    i3 := bank.FindUnitIndex(3); assert bank.units[i3] == 3;
+    i4 := bank.FindUnitIndex(4); assert bank.units[i4] == 4;
+    bank.RemoveUnitByIndex(i4); assert bank.units == [1,2,3];
+    bank.AddUnit(4); assert bank.units == [1,2,3,4];
+    available := bank.GetAvailableUnits(2); assert bank.units == [1,2,3,4];
+}
+
+
+    
