verification_finalised/bank/bank2.dfy
@@ -1,0 +1,79 @@
+//-----------------------------------------------------------------------------
+// Blood Bank Class
+//-----------------------------------------------------------------------------
+
+// Blood bank class. Contains a sequence of integers, each 
+// representing a hypothetical blood unit. The operations are defined
+// on this sequence are all guarenteed to preserve the valid state of the 
+// system. These operations include: adding units, removing units, querying the
+// units, sorting the units.
+class {:autocontracts} BloodBank {
+
+    // Sequence of integers representing blood units
+    var units: seq<int>;
+
+    // Determines wether the blood bank is in a valid state
+    // The units must be distinct integers and the blood bank 
+    // can only hold between 0 and 100,000 units 
+    predicate Valid() 
+    reads this;
+    {
+        0 <= |units| <= 100000 &&
+        forall i, j :: (0<=i<|units| && 0<=j<|units| && i != j) ==> units[i] != units[j]
+    }
+
+    // Constructor for blood bank takes no arguments and creates
+    // an empty units sequence
+    constructor () 
+    modifies this;
+    ensures |units| == 0; 
+    {
+        units := [];
+    }
+
+    // Predicate to determine if the bank is full or not
+    predicate Full()
+    reads this;
+    {
+        |units| == 100000
+    }
+
+    // Add an new unit to the system
+    // This method ensures that an employee cannot add a unit if the storage is full,
+    // and that the same unit cannot be added to the bank twice.
+    method AddUnit(unit: int) 
+    requires !Full(); 
+    requires unit !in units;
+    ensures unit in units;
+    ensures units == old(units) + [unit]
+    {
+        var index, limit := 0, |units|;
+        while unit > units[index] && index < limit
+        decreases limit - index;
+        invariant index <= limit;
+        invariant forall i :: 0<=i<index ==> units[i] < unit;
+        {
+            index := index + 1;           
+        }
+        if index == limit 
+        { units := units[..index] + [unit]; }
+        else 
+        { units := units[..index] + [unit] + units[index+1..]; }
+    }
+}
+
+method Main() {
+    // Initialise blood bank and index variables
+    var bank: BloodBank;
+    var i1: int, i2: int, i3: int, i4: int, i5: int;
+    var f1: seq<int>, f2: seq<int>;
+    var available: seq<int>;
+    var order: seq<int>;
+
+    // Test 1: Tests functionality of AddUnit, FindUnitIndex and RemoveUnitByIndex
+    bank := new BloodBank();
+    bank.AddUnit(1); //assert bank.units == [1];
+    bank.AddUnit(5); //assert bank.units == [1,2];
+    bank.AddUnit(2); //assert bank.units == [1,2,5];
+    print bank.units;
+}
